`2.2.2`
a) 
6 8 14 17 23 - 4c 0s
6 8 14 17 23 - 3c 0s
6 8 14 17 23 - 2c 0s
6 8 14 17 23 - 1c 0s
10c
(n-1)+(n-2) + 1 = SUM from i=0 to n-1 of i = m * (m + 1 ) / 2 = (n-1)*n / 2 = 4*5/2 = 10
sum for n = n*(n+1)/2
sum for n +1 = sum for n + (n+1) = n*(n+1)/2 + (n+1) = (2*(n+1) + n*(n+1))/2 = (n+1)(n+1 +1) /2 

b)
17 23 14 6 8 - 1s
6 23 14 17 8 - 1s
6 8 14 17 23 - 1s
6 8 14 17 23 - 0s
2s
c) 23, 17, 14, 8, 6
5s

`2.2.2`
min comparisons = max comparisons = sum from i=1 to n-1 of i
min swaps = 0, max swaps = n

`2.2.5`
Compares.

`2.3.1`

a

```latex
n = 1
\sum\limits_{i=1}^n i = \frac {n(n+1)} {2}
``` 
base : 1 = 1 (1+1) /2 = 1
induct : n + 1 + sum = n + 1 + n(n+1)/2 (by ind) = m(m+1)/2, where m = n + 1

`2.3.2`
sum j 1 n sum i 1 j = n(n+1) (n+2)/6
base: 1 = 1 + 2 + 3 / 6 = 1

sum j 1 (n+1) sum i 1 j = sum i 1 (n+1) + sum j 1 n sum i 1 j = (n+1)(n+2)/2 + n(n+1)(n+2)/6 = 
= m (m+1) / 2 + (m-1) m (m+1) 6 = m (m+1) (1/2 + m-1 /6) = m (m+1) (3 + m - 1) /6 = m (m+1)(2 + m)/6
 
`2.3.3`
a odd
b even
c odd

`2.3.4`
 




